Attempts at integrating local trace and histroy into logical relation

rupicola/io/ExpRel.fst
@@ -12,7 +12,7 @@ open Trace
 type io_cexp (t:qType) =
   io (get_Type t)
 
-type io_oexp (g:typ_env) (t:qType) =
+let io_oexp (g:typ_env) (t:qType) =
   eval_env g -> io (get_Type t)
 
 (** Cross Language Binary Logical Relation between F* and STLC expressions
@@ -45,7 +45,7 @@ and (⦂) (t:qType) (p:history * io_cexp t * closed_exp) : Tot Type0 (decreases 
       (forall (e':closed_exp). steps e e' h lt ==>  t ∋ (h++lt, fs_r, e'))**)
   forall lt (e':closed_exp).
     steps e e' h lt ==> irred e' (h++lt) ==>
-    (exists fs_r. t ∋ (h++lt, fs_r, e') /\ (forall p. theta fs_e h p ==> p lt fs_r))
+    (exists fs_r. t ∋ (h++lt, fs_r, e'))// /\ (forall p. theta fs_e h p ==> p lt fs_r))
                            (** TODO: ^^^^^^^^^^^^^^^^^^^^^^^^^^^^^^^^^^ check this **)
 
 (** Section 8.1: https://www.cs.uoregon.edu/research/summerschool/summer24/lectures/Ahmed.pdf **)
@@ -85,7 +85,7 @@ let rec lem_values_are_values t h fs_e (e:closed_exp) :
 
 let (∽) (#g:typ_env) #b (h:history) (fsG:eval_env g) (s:gsub g b) : Type0 =
   forall (x:var). Some? (g x) ==>
-    Some?.v (g x) ∋ (h, index fsG x, s x)
+    Some?.v (g x) ⦂ (h, io_return (index fsG x), s x)
   (**  TODO      ^^^ not like in Amal's work. she uses an exp relation **)
 
 (** Cross Language Binary Logical Relation between F* and STLC expressions
@@ -95,11 +95,12 @@ let equiv (#g:typ_env) (t:qType) (fs_e:io_oexp g t) (e:exp) : Type0 =
   forall b (s:gsub g b) (fsG:eval_env g) (h:history).
     fsG `(∽) h` s ==> t ⦂ (h, fs_e fsG, gsubst s e)
 
-let equiv_closed (#t:qType) (fs_e:io_cexp t) (e:exp) : Type0 =
+let equiv_closed (#t:qType) (fs_e:io_cexp t) (e:closed_exp) : Type0 =
   equiv #empty t (fun _ -> fs_e) e
 
-let safety (#t:qType) (fs_e:io_cexp t) (e:exp) : Lemma
-  (requires (equiv_closed fs_e e))
+let safety (#t:qType) (fs_e:io_cexp t) (e:closed_exp) : Lemma
+  (requires equiv_closed fs_e e)
+  //(requires (forall h. t ⦂ (h, fs_e, e))) 
   (ensures (forall h. safe e h)) =
   introduce forall h (e':closed_exp) (lt:local_trace h).
     steps e e' h lt ==> is_value e' \/ can_step e' (h++lt) with begin
@@ -109,7 +110,7 @@ let safety (#t:qType) (fs_e:io_cexp t) (e:exp) : Lemma
           fsG `(∽) h` s ==> t ⦂ (h, fs_e, gsubst s e)
         with  true gsub_empty empty_eval h;
         assert (t ⦂ (h, fs_e, e));
-        eliminate exists fs_r. t ∋ (h++lt, fs_r, e') /\ (forall p. theta fs_e h p ==> p lt fs_r)
+        eliminate exists fs_r. t ∋ (h++lt, fs_r, e') ///\ (forall p. theta fs_e h p ==> p lt fs_r)
         returns is_value e' with _. begin
           assert (t ∋ (h++lt, fs_r, e'));
           lem_values_are_values t (h++lt) fs_r e';
@@ -123,18 +124,22 @@ let (≈) (#g:typ_env) (#t:qType) (fs_v:io_oexp g t) (e:exp) : Type0 =
   equiv #g t fs_v e
 
 (** Equiv closed terms **)
-let equiv_closed_terms (#t:qType) (fs_e:io (get_Type t)) (e:closed_exp) :
+let equiv_closed_terms (#t:qType) (fs_e:io_cexp t) (e:closed_exp) :
   Lemma (requires equiv #empty t (fun _ -> fs_e) e)
-        (ensures  t ⦂ (fs_e, e)) =
-  eliminate forall b (s:gsub empty b) (fsG:eval_env empty).
-    fsG ∽ s ==> t ⦂ ((fun _ -> fs_e) fsG, gsubst s e) with true gsub_empty empty_eval
+        (ensures (forall h. t ⦂ (h, fs_e, e))) =
+  eliminate forall b (s:gsub empty b) (fsG:eval_env empty). forall (h:history).
+    fsG `(∽) h` s ==> t ⦂ (h, (fun _ -> fs_e) fsG, gsubst s e) with true gsub_empty empty_eval
 
-let lem_equiv_exp_are_equiv (g:typ_env) (#t:qType) (fs_e:io (get_Type t)) (e:closed_exp) :
-  Lemma (requires t ⦂ (fs_e, e))
-        (ensures  equiv #empty t (fun _ -> fs_e) e) =
-  introduce forall b (s:gsub empty b) (fsG:eval_env empty).
-    fsG ∽ s ==> t ⦂ ((fun _ -> fs_e) fsG, gsubst s e) with begin
-    assert (gsubst s e == e)
+let lem_equiv_exp_are_equiv (g:typ_env) (#t:qType) (fs_e:io_cexp t) (e:closed_exp) :
+  Lemma (requires (forall h. t ⦂ (h, fs_e, e)))
+        (ensures equiv #empty t (fun _ -> fs_e) e) =
+  introduce forall b (s:gsub empty b) (fsG:eval_env empty) (h':history).
+    fsG `(∽) h'` s ==> t ⦂ (h', (fun _ -> fs_e) fsG, gsubst s e) with begin
+    introduce fsG `(∽) h'` s ==> t ⦂ (h', (fun _ -> fs_e) fsG, gsubst s e) with _. begin
+      assert (gsubst s e == e);
+      assert ((fun _ -> fs_e) fsG == fs_e);
+      eliminate forall h. t ⦂ (h, fs_e, e) with h'
+    end
   end
 
 (** Rules **)
@@ -142,156 +147,182 @@ let lem_equiv_exp_are_equiv (g:typ_env) (#t:qType) (fs_e:io (get_Type t)) (e:clo
 let equiv_unit g
   : Lemma ((fun (_:eval_env g) -> io_return ()) `equiv qUnit` EUnit)
   =
-  introduce forall b (s:gsub g b) fsG. fsG ∽ s ==> qUnit ⦂ (io_return (), gsubst s EUnit) with begin
+  introduce forall b (s:gsub g b) fsG h. fsG `(∽) h` s ==> qUnit ⦂ (h, io_return (), gsubst s EUnit) with begin
     introduce _ ==> _ with _. begin
-      assert (qUnit ∋ ((), EUnit));
-      lem_values_are_expressions qUnit () EUnit
+      assert (qUnit ∋ (h, (), EUnit));
+      lem_values_are_expressions qUnit h () EUnit
     end
   end
 
 let equiv_true g
   : Lemma ((fun (_:eval_env g) -> io_return true) `equiv qBool` ETrue)
   =
-  introduce forall b (s:gsub g b) fsG. fsG ∽ s ==> qBool ⦂ (io_return true, gsubst s ETrue) with begin
+  introduce forall b (s:gsub g b) fsG h. fsG `(∽) h` s ==> qBool ⦂ (h, io_return true, gsubst s ETrue) with begin
     introduce _ ==> _ with _. begin
-      assert (qBool ∋ (true, ETrue));
-      lem_values_are_expressions qBool true ETrue
+      assert (qBool ∋ (h, true, ETrue));
+      lem_values_are_expressions qBool h true ETrue
     end
   end
 
 let equiv_false g
   : Lemma ((fun (_:eval_env g) -> io_return false) `equiv qBool` EFalse)
   =
-  introduce forall b (s:gsub g b) fsG. fsG ∽ s ==> qBool ⦂ (io_return false, gsubst s EFalse) with begin
+  introduce forall b (s:gsub g b) fsG h. fsG `(∽) h` s ==> qBool ⦂ (h, io_return false, gsubst s EFalse) with begin
     introduce _ ==> _ with _. begin
-      assert (qBool ∋ (false, EFalse));
-      lem_values_are_expressions qBool false EFalse
+      assert (qBool ∋ (h, false, EFalse));
+      lem_values_are_expressions qBool h false EFalse
     end
   end
 
 let equiv_var g (x:var{Some? (g x)})
   : Lemma ((fun (fsG:eval_env g) -> io_return (index fsG x)) ≈ EVar x)
   =
-  introduce forall b (s:gsub g b) fsG. fsG ∽ s ==> Some?.v (g x) ⦂ (io_return (index fsG x), gsubst s (EVar x)) with begin
+  introduce forall b (s:gsub g b) fsG h. fsG `(∽) h` s ==> Some?.v (g x) ⦂ (h, io_return (index fsG x), gsubst s (EVar x)) with begin
     introduce _ ==> _ with _. begin
-      assert (Some?.v (g x) ∋ (index fsG x, s x));
-      lem_values_are_expressions (Some?.v (g x)) (index fsG x) (s x)
+      assert (Some?.v (g x) ⦂ (h, io_return (index fsG x), s x))
+      //lem_values_are_expressions (Some?.v (g x)) h (index fsG x) (s x)
     end
   end
 
-let equiv_lam #g (t1:qType) (t2:qType) (f:fs_oexp g (t1 ^-> t2)) (body:exp) : Lemma
+//#push-options "--split_queries always --fuel 3000 --z3rlimit 32"
+let equiv_lam #g (t1:qType) (t2:qType) (f:io_oexp g (t1 ^-> t2)) (body:exp) : Lemma
   (requires (fun (fsG:eval_env (extend t1 g)) -> io_bind (f (tail #t1 fsG)) (fun f -> f (hd fsG))) ≈ body)
-  (ensures f ≈ (ELam body)) = admit ()
-  (*lem_fv_in_env_lam g t1 body;
+  (ensures f ≈ (ELam body)) =
+  lem_fv_in_env_lam g t1 body;
   let g' = extend t1 g in
-  introduce forall b (s:gsub g b) fsG. fsG ∽ s ==> (t1 ^-> t2) ⦂ (f fsG, gsubst s (ELam body)) with begin
+  introduce forall b (s:gsub g b) fsG h. fsG `(∽) h` s ==> (t1 ^-> t2) ⦂ (h, f fsG, gsubst s (ELam body)) with begin
     introduce _ ==> _ with _. begin
       let body' = subst (sub_elam s) body in
       assert (gsubst s (ELam body) == ELam body');
-      introduce forall (v:value) (fs_v:get_Type t1). t1 ∋ (fs_v, v) ==>  t2 ⦂ (f fsG fs_v, subst_beta v body') with begin
+      introduce forall (v:value) (fs_v:get_Type t1) (lt_v:local_trace h). t1 ∋ ((h++lt_v), fs_v, v) ==> t2 ⦂ ((h++lt_v), io_bind (f fsG) (fun f -> f fs_v), subst_beta v body') with begin
         introduce _ ==> _ with _. begin
           let s' = gsub_extend s t1 v in
           let fsG' = stack fsG fs_v in
-          eliminate forall b (s':gsub g' b) (fsG':eval_env g'). fsG' ∽ s' ==>  t2 ⦂ (f (tail #t1 fsG') (hd #t1 #g fsG'), (gsubst s' body))
-            with false s' fsG';
-          assert (fsG ∽ s);
-          assert (stack fsG fs_v ∽ gsub_extend s t1 v);
-          assert (t2 ⦂ (f (tail fsG') (hd fsG'), (gsubst s' body)));
-          assert (hd (stack fsG fs_v) == fs_v);
-          assert (t2 ⦂ (f (tail fsG') fs_v, (gsubst s' body)));
-          assert (t2 ⦂ (f fsG fs_v, (gsubst s' body)));
+          let h' = h++lt_v in
+          eliminate forall b (s':gsub g' b) (fsG':eval_env g') h'. fsG' `(∽) h'` s' ==> t2 ⦂ (h', io_bind (f (tail #t1 fsG')) (fun f -> f (hd #t1 #g fsG')), (gsubst s' body))
+            with false s' fsG' h';
+          assert (fsG `(∽) h` s);
+          assert (forall (x:var). Some? (g x) ==> Some?.v (g x) ⦂ (h, io_return (index fsG x), s x));
+          lem_stack_index fsG fs_v;
+          assert (forall (x:var). Some? (g x) ==> index fsG x == index (stack fsG fs_v) (x+1));
+          assert (forall (x:var). Some? (g x) ==> Some?.v (g x) ⦂ (h, io_return (index (stack fsG fs_v) (x+1)), s x));
+          (*lem_index_tail (stack fsG fs_v);
+          assert (forall (x:var). Some? (g x) ==> index (stack fsG fs_v) (x+1) == index (tail (stack fsG fs_v)) x);
+          assert (forall (x:var). Some? (g x) ==> index fsG x == index (tail (stack fsG fs_v)) x);
+          tail_stack_inveqse fsG fs_v;
+          assert (forall (x:var). Some? (g x) ==> index*)
+          (*introduce forall (x:var). Some? ((extend t1 g) x) ==> Some?.v ((extend t1 g) x) ⦂ (h', io_return (index (stack fsG fs_v) x), (gsub_extend s t1 v) x) with begin
+            introduce Some? ((extend t1 g) x) ==> Some?.v ((extend t1 g) x) ⦂ (h', io_return (index (stack fsG fs_v) x), (gsub_extend s t1 v) x) with _. begin
+              eliminate forall (x:var). Some? (g x) ==> Some?.v (g x) ⦂ (h, io_return (index fsG x), s x) with x;
+              lem_index_tail (stack fsG fs_v);
+              
+              ()
+            end
+          end;*)
+          assume (stack fsG fs_v `(∽) h'` gsub_extend s t1 v); 
+          assert (t2 ⦂ (h', io_bind (f (tail fsG')) (fun f -> f (hd fsG')), (gsubst s' body)));
+          assert ((hd fsG') == fs_v);
+          assert (t2 ⦂ (h', io_bind (f (tail fsG')) (fun f -> f fs_v), (gsubst s' body)));
+          assert (t2 ⦂ (h', io_bind (f fsG) (fun f -> f fs_v), (gsubst s' body)));
           lem_substitution s t1 v body;
-          assert (t2 ⦂ (f fsG fs_v, subst_beta v body'))
+          assert (t2 ⦂ (h', io_bind (f fsG) (fun f -> f fs_v), subst_beta v body'));
+          ()
         end
       end;
-      assert ((t1 ^-> t2) ∋ (f fsG, gsubst s (ELam body)));
-      lem_values_are_expressions (t1 ^-> t2) (f fsG) (gsubst s (ELam body));
-      assert ((t1 ^-> t2) ⦂ (f fsG, gsubst s (ELam body)))
+      let f' : (get_Type t1) -> io (get_Type t2) = fun x -> io_bind (f fsG) (fun f -> f x) in
+      assert ((t1 ^-> t2) ∋ (h, f' , gsubst s (ELam body)));
+      lem_values_are_expressions (t1 ^-> t2) h f' (gsubst s (ELam body));
+      assert ((t1 ^-> t2) ⦂ (h, f fsG, gsubst s (ELam body)))
     end
-  end*)
+  end
+//#pop-options
 
 let equiv_app #g
   (#t1:qType) (#t2:qType)
-  (fs_e1:fs_oexp g (t1 ^-> t2)) (fs_e2:fs_oexp g t1)
+  (fs_e1:io_oexp g (t1 ^-> t2)) (fs_e2:io_oexp g t1)
   (e1:exp) (e2:exp)
   : Lemma
     (requires fs_e1 ≈ e1 /\ fs_e2 ≈ e2)
     (ensures
         (fun fsG -> io_bind (fs_e1 fsG) (fun f -> io_bind (fs_e2 fsG) f))
         ≈
-        (EApp e1 e2))
-  = admit ()
-  (**
-  lem_fv_in_env_app g e1 e2;
-  introduce forall b (s:gsub g b) fsG. fsG ∽ s ==> t2 ⦂ ((fs_e1 fsG) (fs_e2 fsG), gsubst s (EApp e1 e2)) with begin
+        (EApp e1 e2)) = admit ()
+  (*lem_fv_in_env_app g e1 e2;
+  introduce forall b (s:gsub g b) fsG h. fsG `(∽) h` s ==> t2 ⦂ (h, io_bind (fs_e1 fsG) (fun f -> io_bind (fs_e2 fsG) f), gsubst s (EApp e1 e2)) with begin
     let fs_e1 = fs_e1 fsG in
     let fs_e2 = fs_e2 fsG in
-    let fs_e = fs_e1 fs_e2 in
+    let fs_e = io_bind (fs_e1) (fun f -> io_bind fs_e2 f) in
     let e = EApp (gsubst s e1) (gsubst s e2) in
     assert (gsubst s (EApp e1 e2) == e);
     let EApp e1 e2 = e in
-    introduce fsG ∽ s ==>  t2 ⦂ (fs_e, e) with _. begin
-      introduce forall (e':closed_exp). steps e e' /\ irred e' ==> t2 ∋ (fs_e, e') with begin
-        introduce _ ==> t2 ∋ (fs_e, e') with h. begin
-          let steps_e_e' : squash (steps e e') = () in
-          FStar.Squash.map_squash #_ #(squash (t2 ∋ (fs_e, e'))) steps_e_e' (fun steps_e_e' ->
-            safety t1 fs_e2 e2;
+    introduce fsG `(∽) h` s ==> t2 ⦂ (h, fs_e, e) with _. begin
+      introduce forall lt (e':closed_exp). steps e e' h lt /\ irred e' (h++lt) ==> (exists fs_r. t2 ∋ (h++lt, fs_r, e')) (*/\ (forall p. theta fs_e h p ==> p lt fs_r))*) with begin
+        introduce _ ==> (exists fs_r. t2 ∋ (h++lt, fs_r, e')) (*/\ (forall p. theta fs_e h p ==> p lt fs_r))*) with _. begin
+          let steps_e_e' : squash (steps e e' h lt) = () in
+          FStar.Squash.map_squash #_ #(squash ((exists fs_r. t2 ∋ (h++lt, fs_r, e') (*/\ (forall p. theta fs_e h p ==> p lt fs_r)*)))) steps_e_e' (fun steps_e_e' ->
+            assume (equiv_closed fs_e2 e2);
+            safety #t1 fs_e2 e2;
             let t1_typ = type_quotation_to_typ (get_rel t1) in
             let t2_typ = type_quotation_to_typ (get_rel t2) in
-            let (e11, e2') = destruct_steps_eapp e1 e2 e' steps_e_e' t1_typ t2_typ in
-            assume ((t1 ^-> t2) ∋ (fs_e1, ELam e11)); (** TODO/Cezar: this was working before the refactoring **)
-            introduce True ==>  t1 ∋ (fs_e2, e2') with _. begin
-              assert (t1 ⦂ (fs_e2, e2));
-              assert (steps e2 e2');
-              assert (irred e2')
+            assume (forall h'. sem_expr_shape (TArr t1_typ t2_typ) e1 h');
+            let (e11, e2', (| lt2, (| lt1, lt3 |) |)) = destruct_steps_eapp e1 e2 e' h lt steps_e_e' t1_typ t2_typ in
+            let fs_e1' : (get_Type t1) -> io (get_Type t2) = fun x -> io_bind fs_e1 (fun f -> f x) in
+            assume ((t1 ^-> t2) ∋ ((h++lt2)++lt1, fs_e1', ELam e11)); (** TODO/Cezar: this was working before the refactoring **)
+            introduce True ==> exists fs_r2. t1 ∋ (h++lt2, fs_r2, e2') with _. begin
+              assert (t1 ⦂ (h, fs_e2, e2));
+              assert (steps e2 e2' h lt2);
+              assume (irred e2' (h++lt2))
             end;
-            eliminate forall (v:value) (fs_v:get_Type t1). t1 ∋ (fs_v, v) ==>
-              t2 ⦂ (fs_e1 fs_v, subst_beta v e11)
-            with e2' fs_e2;
-            assert (t2 ⦂ (fs_e, subst_beta e2' e11));
-            assert (t2 ∋ (fs_e, e'))
+            assert (exists fs_r2. t1 ∋ (h++lt2, fs_r2, e2'));
+            eliminate exists fs_r2. t1 ∋ (h++lt2, fs_r2, e2') returns (exists fs_r2. t2 ∋ (h++lt, fs_r2, e')) with  _. begin 
+              (*eliminate forall (v:value) (fs_v:get_Type t1) (lt_v:local_trace h). t1 ∋ (h++lt_v, fs_v, v) ==>
+                t2 ⦂ (h++lt_v, io_bind (fs_e1) (fun f -> f fs_v), subst_beta v e11)
+              with e2' fs_r2 lt2;*)
+              assume (t2 ⦂ (h++lt2, fs_e, subst_beta e2' e11));
+              assert (t2 ∋ (h++lt, fs_r2, e'))
+           end
           )
         end
       end
     end
-  end **)
+  end*)
 
-let equiv_if #g (#t:qType) (fs_e1:fs_oexp g qBool) (fs_e2:fs_oexp g t) (fs_e3:fs_oexp g t) (e1:exp) (e2:exp) (e3:exp) : Lemma
+let equiv_if #g (#t:qType) (fs_e1:io_oexp g qBool) (fs_e2:io_oexp g t) (fs_e3:io_oexp g t) (e1:exp) (e2:exp) (e3:exp) : Lemma
   (requires fs_e1 ≈ e1 /\ fs_e2 ≈ e2 /\ fs_e3 ≈ e3)
   (ensures (
     (fun fsG ->
       io_bind (fs_e1 fsG) (fun b -> if b then fs_e2 fsG else fs_e3 fsG))
     ≈
     (EIf e1 e2 e3))) =
-  admit ()
-  (**
   lem_fv_in_env_if g e1 e2 e3;
-  introduce forall b (s:gsub g b) fsG. fsG ∽ s ==> t ⦂ ((if fs_e1 fsG then fs_e2 fsG else fs_e3 fsG), gsubst s (EIf e1 e2 e3)) with begin
-    (*let fs_e1 = fs_e1 fsG in
-    let fs_e = if fs_e1 then fs_e2 fsG else fs_e3 fsG in
+  introduce forall b (s:gsub g b) fsG h. fsG `(∽) h` s ==> t ⦂ (h, io_bind (fs_e1 fsG) (fun b -> if b then fs_e2 fsG else fs_e3 fsG), gsubst s (EIf e1 e2 e3)) with begin
+    let fs_e1 = fs_e1 fsG in
+    let fs_e = io_bind fs_e1 (fun b -> if b then fs_e2 fsG else fs_e3 fsG) in
     let e = EIf (gsubst s e1) (gsubst s e2) (gsubst s e3) in
     assert (gsubst s (EIf e1 e2 e3) == e);
     let EIf e1 e2 e3 = e in
-    introduce fsG ∽ s ==> t ⦂ (fs_e, e) with _. begin
-      introduce forall (e':closed_exp). steps e e' /\ irred e' ==> t ∋ (fs_e, e') with begin
-        introduce _ ==> t ∋ (fs_e, e') with h. begin
-          let steps_e_e' : squash (steps e e') = () in
-          FStar.Squash.map_squash #_ #(squash (t ∋ (fs_e, e'))) steps_e_e' (fun steps_e_e' ->
-            safety qBool fs_e1 e1;
-            safety t (fs_e2 fsG) e2;
-            safety t (fs_e3 fsG) e3;
-            let e1' = destruct_steps_eif e1 e2 e3 e' steps_e_e' in
-            assert (qBool ∋ (fs_e1, e1'));
-            assert (ETrue? e1' ==> (t ∋ (fs_e2 fsG, e')));
-            assert (EFalse? e1' ==> (t ∋ (fs_e3 fsG, e')));
-            assert (t ∋ (fs_e, e'))
+    introduce fsG `(∽) h` s ==> t ⦂ (h, fs_e, e) with _. begin
+      introduce forall lt (e':closed_exp). steps e e' h lt /\ irred e' (h++lt) ==> (exists fs_r. t ∋ (h++lt, fs_r, e') /\ (forall p. theta fs_e h p ==> p lt fs_r)) with begin
+        introduce _ ==> (exists fs_r. t ∋ (h++lt, fs_r, e') /\ (forall p. theta fs_e h p ==> p lt fs_r)) with _. begin
+          let steps_e_e' : squash (steps e e' h lt) = () in
+          FStar.Squash.map_squash #_ #(squash (exists fs_r. t ∋ (h++lt, fs_r, e') /\ (forall p. theta fs_e h p ==> p lt fs_r))) steps_e_e' (fun steps_e_e' ->
+            assume (equiv_closed fs_e1 e1);
+            safety #qBool fs_e1 e1;
+            assume (equiv_closed (fs_e2 fsG) e2);
+            safety #t (fs_e2 fsG) e2;
+            assume (equiv_closed (fs_e3 fsG) e3);
+            safety #t (fs_e3 fsG) e3;
+            let (e1', (| lt1, (lt2, lt3) |)) = destruct_steps_eif e1 e2 e3 e' h lt steps_e_e' in
+            assert (qBool ⦂ (h, fs_e1, e1));
+            assert (qBool ∋ (h, fs_e1, e1'));
+            assert (ETrue? e1' ==> (t ∋ (h++lt1, fs_e2 fsG, e')));
+            assert (EFalse? e1' ==> (t ∋ (h++lt1, fs_e3 fsG, e')));
+            assert (t ∋ (h++lt, fs_e, e'))
           )
         end
       end
-    end*)
-    admit ()
+    end
   end
-  **)
 
 (**
 let equiv_pair #g (#t1 #t2:qType) (fs_e1:fs_oexp g t1) (fs_e2:fs_oexp g t2) (e1:exp) (e2:exp) : Lemma
